
$$ a_{1}x+b_{1}y = \epsilon_{1}$$
$$a_{2}x+b_{2}y = \epsilon_{2} $$
$|a_{1}$  $b_{1}|$ = $\Delta$ = $a_{1}b_{2}-a_{2}b_{1}$
$|a_{2}$  $b_{2}$| 



$|\varepsilon_{1}$  $b_{1}|$ = $\Delta_{x}$ = $\epsilon_{1}b_{2}-\epsilon_{2}b_{1}$
$|\epsilon_{2}$  $b_{2}$| 


$|a_{1}$  $\epsilon_{1}|$ = $\Delta_{y}$ = $a_{1}\epsilon_{2}-a_{2}\epsilon_{1}$
$|a_{2}$  $\epsilon_{2}$| 

$$x = \frac{\Delta_{x}}{\Delta}$$
$$y = \frac{\Delta_{y}}{\Delta}$$

### 3x3

$$ a_{1}x+b_{1}y+c_{1} = \epsilon_{1}$$
$$a_{2}x+b_{2}y + c{2} = \epsilon_{2} $$
$$a_{3}x+b_{3}y + c{3} = \epsilon_{3} $$

|$a_{1}$  $b_{1}$ $c_{1}$  |
|$a_{2}$  $b_{2}$  $c_{2}$ | = $\Delta$ = $a_{1} b_{2}c_{3}$ + $a_{3}b_{1}c_{2}$  + $a_{2}b_{3}c_{1}$ - $a_{3}b_{2}c_{1}$ - $a_{2}b_{1}c_{3}$ - $a_{1}b_{3}c_{2}$ 
|$a_{3}$  $b_{3}$  $c_{3}$ | 